Extraction/ArmInstExtr.v
@@ -69,5 +69,5 @@ Set Extraction Output Directory ".".
 
 #[warnings="-extraction-remaining-implicit,-extraction-reserved-identifier"]
 Separate Extraction
-  Arm sail_tiny_arm_sem UMPromising_opmodel_pf VMPromising_opmodel_pf
+  Arm sail_tiny_arm_sem UMPromising_opmodel_pf UMPromising_opmodel_fixed_pf VMPromising_opmodel_pf
   X86Inst.X86 sail_tiny_x86_sem x86_tso_opmodel x86_tso_opmodel_eager.
